Coq/exp.v
@@ -1,7 +1,6 @@
 Require Import common.
 Require Import loo_def.
 Require Import decoupling.
-Require Import decoupled_classical_properties.
 Require Import loo_properties.
 Require Import loo_reduction_properties.
 Require Import function_operations.
@@ -19,11 +18,19 @@ Proof.
   inversion H;
     subst.
   match goal with
+  | [H : exp_satisfaction _ _ _ _ |- _ ] =>
+    inversion H;
+      subst;
+      clear H
+  end.
+  match goal with
   | [H : is_exp _ _ |- _] =>
     inversion H;
       subst
-  end.
-  eapply sat_exp with (e':=e2' ⩵ e1');
+  end;
+    eauto with chainmail_db.
+  apply sat_exp.
+  eapply exp_sat with (e':=e2' ⩵ e1');
     eauto with chainmail_db.
   match goal with
   | [ H : _ ∙ _ ⊢ _ ⩵ _ ↪ _ |- _] =>
@@ -179,147 +186,3 @@ Ltac is_exp_auto :=
            auto;
            subst
          end.
-
-Lemma transitive_equality :
-  forall M1 M2 σ0 σ e1 e2, M1 ⦂ M2 ◎ σ0 … σ ⊨ (e1 ⩶ e2) ->
-                      forall e3, M1 ⦂ M2 ◎ σ0 … σ ⊨ (e2 ⩶ e3) ->
-                            M1 ⦂ M2 ◎ σ0 … σ ⊨ (e1 ⩶ e3).
-Proof.
-  intros.
-  repeat match goal with
-         | [H : _ ⦂ _ ◎ _ … _ ⊨ _ |- _] =>
-           inversion H;
-             subst;
-             clear H
-         end.
-  is_exp_auto.
-  repeat match goal with
-         | [H : _ ∙ _ ⊢  (_ ⩵ _) ↪ _ |- _] =>
-           inversion H;
-             subst;
-             clear H
-         end.
-  link_unique_auto.
-  eval_rewrite.
-  eapply sat_exp;
-    eauto with chainmail_db loo_db.
-Qed.
-
-Lemma value_equality_eval :
-  forall M σ v1 v2, M ∙ σ ⊢ (e_val v1 ⩵ e_val v2) ↪ v_true ->
-               v1 = v2.
-Proof.
-  intros.
-  repeat match goal with
-         | [H : _ ∙ _ ⊢ _ ↪ _ |- _ ] =>
-           inversion H;
-             subst;
-             clear H
-         end;
-    auto.
-Qed.
-
-Lemma value_equality :
-  forall M1 M2 σ0 σ v1 v2, M1 ⦂ M2 ◎ σ0 … σ ⊨ (ex_val v1 ⩶ ex_val v2) ->
-                      v1 = v2.
-Proof.
-  intros M1 M2 σ0 σ v1 v2 Hsat;
-    inversion Hsat;
-    subst.
-  is_exp_auto.
-  match goal with
-  | [ H : _ ∙ _ ⊢ (e_val _ ⩵ e_val _) ↪ v_true |- _ ] =>
-    apply value_equality_eval in H
-  end.
-  auto.
-Qed.
-
-Lemma value_reflexivity_eval :
-  forall M σ v, M ∙ σ ⊢ (e_val v ⩵ e_val v) ↪ v_true.
-Proof.
-  intros.
-  apply v_equals with (v:=v);
-    eauto with loo_db.
-Qed.
-
-Lemma value_reflexivity :
-  forall M1 M2 M σ0 σ v, M1 ⋄ M2 ≜ M ->
-                    M1 ⦂ M2 ◎ σ0 … σ ⊨ (ex_val v ⩶ ex_val v).
-Proof.
-  intros.
-  eapply sat_exp with (e':=(e_val v ⩵ e_val v));
-    eauto with chainmail_db.
-  apply value_reflexivity_eval.
-Qed.
-
-Lemma neq_is_nsat_eq_1 :
-  forall M1 M2 σ0 σ e1 e2, M1 ⦂ M2 ◎ σ0 … σ ⊨ (e1 ⩶̸ e2) ->
-                      M1 ⦂ M2 ◎ σ0 … σ ⊭ (e1 ⩶ e2).
-Proof.
-  intros M1 M2 σ0 σ e1 e2 Hneq.
-  apply not_sat_implies_nsat;
-    intro Hcontra.
-  repeat match goal with
-         | [H : _ ⦂ _ ◎ _ … _ ⊨ _ |- _] =>
-           inversion H;
-             subst;
-             clear H
-         end.
-  is_exp_auto.
-  link_unique_auto.
-  match goal with
-  | [H : _ ∙ _ ⊢ neg _ ↪ _  |- _] =>
-    inversion H;
-      subst;
-      clear H
-  end.
-  eval_rewrite.
-  match goal with
-  | [H : _ ∙ _ ⊢ _ ↪ _ |- _ ] =>
-    inversion H
-  end.
-Qed.
-
-Ltac exp_sym_auto :=
-  match goal with
-  | [H : ?M1 ⦂ ?M2 ◎ ?σ0 … ?σ ⊨ (?e1 ⩶ ?e2) |- _] =>
-    notHyp (M1 ⦂ M2 ◎ σ0 … σ ⊨ (e2 ⩶ e1));
-    assert (M1 ⦂ M2 ◎ σ0 … σ ⊨ (e2 ⩶ e1));
-    [apply symmetric_equality; auto|]
-  end.
-
-Ltac exp_trans_auto :=
-  match goal with
-  | [H1 : ?M1 ⦂ ?M2 ◎ ?σ0 … ?σ ⊨ (?e1 ⩶ ?e2),
-          H2 : ?M1 ⦂ ?M2 ◎ ?σ0 … ?σ ⊨ (?e2 ⩶ ?e3) |- _] =>
-    notHyp (M1 ⦂ M2 ◎ σ0 … σ ⊨ (e1 ⩶ e3));
-    assert (M1 ⦂ M2 ◎ σ0 … σ ⊨ (e1 ⩶ e3));
-    [apply transitive_equality with (e2:=e2); auto|]
-  end.
-
-Ltac clean :=
-  repeat match goal with
-         | [H1 : ?P,
-                 H2 : ?P|- _] =>
-           clear H2
-         end.
-
-Ltac exp_auto :=
-  repeat link_unique_auto;
-  repeat eval_rewrite;
-  repeat is_exp_auto;
-  repeat exp_sym_auto;
-  repeat exp_trans_auto;
-  repeat match goal with
-         | [H : ?M1 ⦂ ?M2 ◎ ?σ0 … ?σ ⊨ (ex_val ?v1 ⩶ ex_val ?v2) |- _] =>
-           assert (v1 = v2);
-           [eapply value_equality; eauto|subst; clear H]
-         end;
-  try match goal with
-      | [Hlink : _ ⋄ _ ≜ ?M |- ?M ∙ _ ⊢ (e_val ?v ⩵ e_val ?v) ↪ v_true ] =>
-        eapply value_reflexivity;
-        eauto
-      | [Hlink : _ ⋄ _ ≜ ?M |- ?M ∙ _ ⊢ (e_val ?v ⩵ e_val ?v) ↪ v_true ] =>
-        eapply value_reflexivity_eval;
-        eauto
-      end.
